fold2.v
@@ -913,3 +913,4 @@ Proof.
   apply precise_is_array.
 Qed.
 End reduce.
+
